theories/FOL/ZF.v
@@ -62,42 +62,42 @@ Notation "x ∪ y" := (⋃ {x; y}) (at level 32) : syn.
 Notation  "'σ' x" := (x ∪ {x; x}) (at level 32) : syn.
 
 Definition sub x y :=
-  ∀ $0 ∈ x`[↑] ~> $0 ∈ y`[↑].
+  ∀ $0 ∈ x`[↑] → $0 ∈ y`[↑].
 
 Notation "x ⊆ y" := (sub x y) (at level 34) : syn.
 
 Definition ax_ext :=
-  ∀ ∀ $1 ⊆ $0 ~> $0 ⊆ $1 ~> $1 ≡ $0.
+  ∀ ∀ $1 ⊆ $0 → $0 ⊆ $1 → $1 ≡ $0.
 
 Definition ax_eset :=
   ∀ ¬ ($0 ∈ ∅).
 
 Definition ax_pair :=
-  ∀ ∀ ∀ $0 ∈ {$1; $2} <~> $0 ≡ $1 ∨ $0 ≡ $2.
+  ∀ ∀ ∀ $0 ∈ {$1; $2} ↔ $0 ≡ $1 ∨ $0 ≡ $2.
 
 Definition ax_union :=
-  ∀ ∀ $0 ∈ ⋃ $1 <~> ∃ $0 ∈ $2 ∧ $1 ∈ $0.
+  ∀ ∀ $0 ∈ ⋃ $1 ↔ ∃ $0 ∈ $2 ∧ $1 ∈ $0.
 
 Definition ax_power :=
-  ∀ ∀ $0 ∈ PP $1 <~> $0 ⊆ $1.
+  ∀ ∀ $0 ∈ PP $1 ↔ $0 ⊆ $1.
 
 Definition inductive x :=
-  ∅ ∈ x ∧ ∀ $0 ∈ x`[↑] ~> σ $0 ∈ x`[↑].
+  ∅ ∈ x ∧ ∀ $0 ∈ x`[↑] → σ $0 ∈ x`[↑].
 
 Definition ax_om1 :=
   inductive ω.
 
 Definition ax_om2 :=
-  ∀ inductive $0 ~> ω ⊆ $0.
+  ∀ inductive $0 → ω ⊆ $0.
 
 Definition ax_sep phi :=
-  ∀ ∃ ∀ $0 ∈ $1 <~> $0 ∈ $2 ∧ phi[$0.: Nat.add 3 >> var].
+  ∀ ∃ ∀ $0 ∈ $1 ↔ $0 ∈ $2 ∧ phi[$0.: Nat.add 3 >> var].
 
 Definition fun_rel phi :=
-  ∀ ∀ ∀ phi[$2 .: $1 .: Nat.add 3 >> var] ~> phi[$2 .: $0 .: Nat.add 3 >> var] ~> $1 ≡ $0.
+  ∀ ∀ ∀ phi[$2 .: $1 .: Nat.add 3 >> var] → phi[$2 .: $0 .: Nat.add 3 >> var] → $1 ≡ $0.
 
 Definition ax_rep phi :=
-  fun_rel phi ~> ∀ ∃ ∀ $0 ∈ $1 <~> ∃ $0 ∈ $3 ∧ phi[$0 .: $1 .: Nat.add 4 >> var].
+  fun_rel phi → ∀ ∃ ∀ $0 ∈ $1 ↔ ∃ $0 ∈ $3 ∧ phi[$0 .: $1 .: Nat.add 4 >> var].
 
 (* Hereditarily finite set theory *)
 
@@ -132,13 +132,13 @@ Definition ax_refl :=
   ∀ $0 ≡ $0.
 
 Definition ax_sym :=
-  ∀ ∀ $1 ≡ $0 ~> $0 ≡ $1.
+  ∀ ∀ $1 ≡ $0 → $0 ≡ $1.
 
 Definition ax_trans :=
-  ∀ ∀ ∀ $2 ≡ $1 ~> $1 ≡ $0 ~> $2 ≡ $0.
+  ∀ ∀ ∀ $2 ≡ $1 → $1 ≡ $0 → $2 ≡ $0.
 
 Definition ax_eq_elem :=
-  ∀ ∀ ∀ ∀ $3 ≡ $1 ~> $2 ≡ $0 ~> $3 ∈ $2 ~> $1 ∈ $0.
+  ∀ ∀ ∀ ∀ $3 ≡ $1 → $2 ≡ $0 → $3 ∈ $2 → $1 ∈ $0.
 
 (* List of HF axioms plus equality axioms *)
 
