theories/FOL/FST.v
@@ -39,18 +39,18 @@ Notation "∅" := (func FST_func_sig eset ([])) : syn.
 Notation "x ::: y" := (func FST_func_sig adj ([x; y])) (at level 31) : syn.
 
 Definition sub x y :=
-  ∀ $0 ∈ x`[↑] ~> $0 ∈ y`[↑].
+  ∀ $0 ∈ x`[↑] → $0 ∈ y`[↑].
 
 Notation "x ⊆ y" := (sub x y) (at level 34) : syn.
 
 Definition ax_ext :=
-  ∀ ∀ $1 ⊆ $0 ~> $0 ⊆ $1 ~> $1 ≡ $0.
+  ∀ ∀ $1 ⊆ $0 → $0 ⊆ $1 → $1 ≡ $0.
 
 Definition ax_eset :=
   ∀ ¬ ($0 ∈ ∅).
 
 Definition ax_adj :=
-  ∀ ∀ ∀ $0 ∈ $1 ::: $2 <~> $0 ≡ $1 ∨ $0 ∈ $2.
+  ∀ ∀ ∀ $0 ∈ $1 ::: $2 ↔ $0 ≡ $1 ∨ $0 ∈ $2.
 
 (* Finite set theory *)
 
@@ -59,8 +59,8 @@ Definition FST :=
 
 Definition ax_ind phi :=
   phi[∅..]
-   ~> (∀ ∀ phi[$0 .: (fun n => $(2+n))] ~> phi[$1 .: (fun n => $(2+n))] ~> phi[$0 ::: $1 .: (fun n => $(2+n))])
-   ~> ∀ phi.
+   → (∀ ∀ phi[$0 .: (fun n => $(2+n))] → phi[$1 .: (fun n => $(2+n))] → phi[$0 ::: $1 .: (fun n => $(2+n))])
+   → ∀ phi.
 
 Inductive FSTI : form -> Prop :=
 | FST_base phi : In phi FST -> FSTI phi
@@ -72,13 +72,13 @@ Definition ax_refl :=
   ∀ $0 ≡ $0.
 
 Definition ax_sym :=
-  ∀ ∀ $1 ≡ $0 ~> $0 ≡ $1.
+  ∀ ∀ $1 ≡ $0 → $0 ≡ $1.
 
 Definition ax_trans :=
-  ∀ ∀ ∀ $2 ≡ $1 ~> $1 ≡ $0 ~> $2 ≡ $0.
+  ∀ ∀ ∀ $2 ≡ $1 → $1 ≡ $0 → $2 ≡ $0.
 
 Definition ax_eq_elem :=
-  ∀ ∀ ∀ ∀ $3 ≡ $1 ~> $2 ≡ $0 ~> $3 ∈ $2 ~> $1 ∈ $0.
+  ∀ ∀ ∀ ∀ $3 ≡ $1 → $2 ≡ $0 → $3 ∈ $2 → $1 ∈ $0.
 
 Definition FSTeq :=
   ax_refl :: ax_sym :: ax_trans :: ax_eq_elem :: FST.
